ADTExamples/QueryStructure/Bookstore.v
@@ -1,11 +1,15 @@
 Require Import String Omega List FunctionalExtensionality Ensembles
-        Computation ADT ADTRefinement ADTNotation QueryStructureSchema
-        BuildADTRefinements QueryQSSpecs InsertQSSpecs EmptyQSSpecs
-        QueryStructure GeneralInsertRefinements ListInsertRefinements
-        GeneralQueryRefinements ListQueryRefinements
+        Computation ADT ADTRefinement ADTNotation BuildADTRefinements
+        QueryStructureSchema QueryStructure
+        QueryQSSpecs InsertQSSpecs EmptyQSSpecs
+        GeneralInsertRefinements GeneralQueryRefinements
+        GeneralQueryStructureRefinements
+        ListQueryRefinements ListInsertRefinements
+        ListQueryStructureRefinements
         ProcessScheduler.AdditionalLemmas.
 
 Section BookStoreExamples.
+  Require Import QueryStructureNotations.
 
   (* Our bookstore has two relations (tables):
      - The [Books] relation contains the books in the
@@ -24,8 +28,6 @@ Section BookStoreExamples.
      constraint.
    *)
 
-  Open Scope QSSchema.
-
   Definition BookStoreSchema :=
     Query Structure Schema
       [ relation "Books" has
@@ -38,25 +40,9 @@ Section BookStoreExamples.
     "Date" :: nat> ]
       enforcing [attribute "ISBN" of "Orders" references "Books"].
 
-  Definition Books := GetRelationKey BookStoreSchema "Books".
-  Definition Orders := GetRelationKey BookStoreSchema "Orders".
-
-  Definition Author := GetAttributeKey Books "Author".
-  Definition Title := GetAttributeKey Books "Title".
-  Definition ISBN := GetAttributeKey Books "ISBN".
-
-  Definition oISBN := GetAttributeKey Orders "ISBN".
-  Definition Date := GetAttributeKey Orders "Date".
-
-  Definition BookStoreRefRep := QueryStructure BookStoreSchema.
-
-  Definition BookSchemaHeading :=
-    QSGetNRelSchemaHeading BookStoreSchema Books.
-  Definition OrderSchemaHeading :=
-    QSGetNRelSchemaHeading BookStoreSchema Orders.
-
-  Definition Book := @Tuple BookSchemaHeading.
-  Definition Order := @Tuple OrderSchemaHeading.
+  (* Aliases for the tuples contained in Books and Orders, respectively. *)
+  Definition Book := TupleDef BookStoreSchema "Books".
+  Definition Order := TupleDef BookStoreSchema "Orders".
 
   (* Our bookstore has two mutators:
      - [PlaceOrder] : Place an order into the 'Orders' table
@@ -66,12 +52,6 @@ Section BookStoreExamples.
      - [GetTitles] : The titles of books written by a given author
      - [NumOrders] : The number of orders for a given author
    *)
-
-  Local Open Scope ADTSig_scope.
-  Local Open Scope QueryStructure_scope.
-  Local Open Scope Schema.
-  Local Open Scope QuerySpec.
-  Local Open Scope string.
 
   Definition BookStoreSig : ADTSig :=
     ADTsignature {
@@ -86,56 +66,28 @@ Section BookStoreExamples.
     QueryADTRep BookStoreSchema {
       const "InitBookstore" (_ : unit) : rep := empty,
 
-      (* [PlaceOrder] : Place an order into the 'Orders' table *)
       update "PlaceOrder" ( o : Order ) : unit :=
-          Insert o into Orders,
+          Insert o into "Orders",
 
-      (* [AddBook] : Add a book to the inventory *)
       update "AddBook" ( b : Book ) : unit :=
-          Insert b into Books ,
+          Insert b into "Books" ,
 
-      (* [GetTitles] : The titles of books written by a given author *)
       query "GetTitles" ( author : string ) : list string :=
-        For (b in Books)
-        Where (author = b!Author)
-        Return (b!Title),
+        For (b in "Books")
+        Where (author = b!"Author")
+        Return (b!"Title"),
 
-      (* [NumOrders] : The number of orders for a given author *)
        query "NumOrders" ( author : string ) : nat :=
-          Count (For (o in Orders) (b in Books)
-                 Where (author = b!Author)
-                 Where (b!ISBN = o!oISBN)
-                 Return o!oISBN)
+          Count (For (o in "Orders") (b in "Books")
+                 Where (author = b!"Author")
+                 Where (b!"ISBN" = o!"ISBN")
+                 Return o!"ISBN")
   }.
 
-  Local Close Scope QueryStructureParsing_scope.
-  Local Close Scope QuerySpec.
-  Local Open Scope QueryStructure_scope.
-
-  Definition BookStoreListImpl_SiR or (nr : list Book * list Order) : Prop :=
-    EnsembleListEquivalence (GetUnConstrRelation or Books) (fst nr)
-    /\ EnsembleListEquivalence (GetUnConstrRelation or Orders) (snd nr).
-
-  Instance ISBN_attr_dec :
-    List_Query_eq (map (Domain BookSchemaHeading) ["ISBN"]%SchemaConstraints).
-  eauto with typeclass_instances.
-  Defined.
-
-  Instance Title_Author_attr_dec :
-    List_Query_eq (map (Domain BookSchemaHeading) ["Title";"Author"]%SchemaConstraints).
-  eauto with typeclass_instances.
-  Defined.
-
-  Lemma EnsembleListEquivalence_Empty :
-    forall qsSchema Ridx,
-      EnsembleListEquivalence
-        (GetUnConstrRelation (DropQSConstraints (QSEmptySpec qsSchema))
-                             Ridx) [].
-  Proof.
-    intros; rewrite GetRelDropConstraints; simpl; split; simpl; intros;
-    unfold GetRelation, In in *;
-    rewrite Build_EmptyRelation_IsEmpty in *; simpl in *; auto.
-  Qed.
+  Definition BookStoreListImpl_SiR
+             (or : UnConstrQueryStructure BookStoreSchema)
+             (nr : list Book * list Order) : Prop :=
+    or ! "Books" ≃ fst nr /\ or ! "Orders" ≃ snd nr.
 
   Definition BookStore :
     Sharpened BookStoreSpec.
@@ -145,118 +97,23 @@ Section BookStoreExamples.
     (* Step 1: Drop the constraints on the tables. From the perspective
       of a client of a sharpened ADT the invariants will still hold,
       since ADT refinement preserves the simulation relation. *)
-    hone representation using (@DropQSConstraints_SiR BookStoreSchema).
+    start honing QueryStructure.
 
-    drop constraints from insert "PlaceOrder".
-    drop constraints from insert "AddBook".
-    drop constraints from query "GetTitles".
-    drop constraints from query "NumOrders".
-
-    (* Step 4: Switch to an implementation of the representation
-       type as a pair of lists of tuples. *)
-    hone representation using BookStoreListImpl_SiR.
-
-    (* Step 5: Implement the [GetTitles] observer for the pair of lists
-     representation. *)
-    hone method "GetTitles".
-    {
-      unfold BookStoreListImpl_SiR in *; split_and.
-      setoid_rewrite refineEquiv_pick_ex_computes_to_and.
-      simplify with monad laws.
-      implement queries for lists.
-      setoid_rewrite refineEquiv_pick_pair_pair.
-      setoid_rewrite refineEquiv_pick_eq'.
-      repeat (rewrite refine_pick_val; [simplify with monad laws | eassumption]).
-      finish honing.
-    }
-
-    (* Step 6: Implement the [NumOrders] observer for the pair of lists
-     representation. *)
-    hone method "NumOrders".
-    {
-      unfold BookStoreListImpl_SiR in *; split_and.
-      (* We first swap the order of the 'fors' to make the
+    (* Step 2: We first swap the order of the 'For's to make the
          implementation more efficient. *)
-      setoid_rewrite refineEquiv_pick_ex_computes_to_and.
-      simplify with monad laws.
-      rewrite Equivalent_Swap_In.
+
+    hone method "NumOrders".
+    { rewrite Equivalent_Swap_In;
       rewrite refine_Query_For_In_Equivalent;
-        [ | apply Equivalent_Swap_In_Where with (qs := _)]; cbv beta.
-      (* Now implement the list query. *)
-      implement queries for lists.
-      setoid_rewrite refineEquiv_pick_pair_pair.
-      setoid_rewrite refineEquiv_pick_eq'.
-      repeat (rewrite refine_pick_val; [simplify with monad laws | eassumption]).
-      rewrite map_length.
-      finish honing.
-    }
+        [ | apply Equivalent_Swap_In_Where with (qs := _)]; cbv beta;
+        finish honing. }
 
-    (* Step 7: Implement the [AddBook] mutator for the pair of lists
-     representation. *)
-    hone method "AddBook".
-    {
-      setoid_rewrite refineEquiv_split_ex.
-      unfold BookStoreListImpl_SiR in *; split_and.
-      setoid_rewrite refineEquiv_pick_computes_to_and.
-      simplify with monad laws.
-      setoid_rewrite refine_unused_key_check
-      with (attr_eq_dec' := ISBN_attr_dec)
-             (attr_eq_dec := _); eauto.
-      simplify with monad laws.
-      setoid_rewrite refine_unused_key_check'
-      with (attr_eq_dec' := ISBN_attr_dec)
-             (attr_eq_dec := _); eauto.
-      simplify with monad laws.
-      rewrite refine_pick_eq_ex_bind; simpl.
-      rewrite refineEquiv_pick_pair_pair.
-      setoid_rewrite refineEquiv_pick_eq'.
-      simplify with monad laws.
-      Split Constraint Checks.
-      implement insert for lists.
-      unfold Orders, Books; congruence.
-      repeat (rewrite refine_pick_val; [rewrite refineEquiv_bind_unit | eassumption]); reflexivity.
-    }
+    (* Step 3: Switch to an implementation of the representation
+       type as a pair of lists of tuples. *)
 
-    (* Step 7: Implement the [PlaceOrder] mutator for the pair of lists
-     representation. *)
-    hone method "PlaceOrder".
-    {
-      unfold BookStoreListImpl_SiR in *; split_and.
-      setoid_rewrite refineEquiv_split_ex.
-      setoid_rewrite refineEquiv_pick_computes_to_and.
-      setoid_rewrite refine_foreign_key_check with
-                     (P_dec := _); eauto.
-      simplify with monad laws.
-      rewrite refine_pick_eq_ex_bind.
-      rewrite refineEquiv_pick_pair_pair.
-      setoid_rewrite refineEquiv_pick_eq'.
-      simplify with monad laws; simpl.
-      Split Constraint Checks; simpl.
-      setoid_rewrite ImplementListInsert_neq; eauto.
-      simplify with monad laws.
-      rewrite H;  setoid_rewrite ImplementListInsert_eq; eauto.
-      simplify with monad laws.
-      reflexivity.
-      unfold Orders, Books; congruence.
-      rewrite H.
-      repeat (rewrite refine_pick_val; [rewrite refineEquiv_bind_unit | eassumption]); reflexivity.
-    }
+    implement using lists under BookStoreListImpl_SiR.
 
-    (* Step 8: Implement the [InitBookstore] constructor.*)
-    hone constructor "InitBookstore".
-    {
-      unfold BookStoreListImpl_SiR, DropQSConstraints_SiR.
-    repeat setoid_rewrite refineEquiv_pick_ex_computes_to_and.
-    repeat setoid_rewrite refineEquiv_pick_eq'.
-    simplify with monad laws.
-    rewrite refineEquiv_pick_pair.
-    repeat (rewrite refine_pick_val;
-            [simplify with monad laws
-             | apply EnsembleListEquivalence_Empty]).
-    subst_body; higher_order_1_reflexivity.
-    }
-
-    (* Step 9: Profit. :) *)
+    (* Step 4: Profit. :) *)
 
     finish sharpening.
   Defined.
