ADTExamples/QueryStructure/GeneralQueryStructureRefinements.v
@@ -1,0 +1,18 @@
+Require Import String Omega List FunctionalExtensionality Ensembles
+        Computation ADT ADTRefinement ADTNotation BuildADTRefinements
+        QueryStructureSchema QueryStructure
+        QueryQSSpecs InsertQSSpecs EmptyQSSpecs
+        GeneralInsertRefinements GeneralQueryRefinements.
+
+Tactic Notation "start" "honing" "QueryStructure" :=
+  match goal with
+      |- context [@BuildADT (QueryStructure ?Rep) _ _ _ _] =>
+      hone representation using (@DropQSConstraints_SiR Rep);
+        repeat (match goal with
+                    |- context [(meth ?R (_ : rep , _ : _ ) : _ :=
+                                   {_ | forall or : QueryStructure _,
+                                          DropQSConstraints_SiR or _ -> _})%methDef] =>
+                    first [ drop constraints from query R
+                          | drop constraints from insert R ]
+                end)
+    end.
