ADTExamples/QueryStructure/ListQueryStructureRefinements.v
@@ -1,0 +1,54 @@
+Require Import String Omega List FunctionalExtensionality Ensembles
+        Computation ADT ADTRefinement ADTNotation QueryStructureSchema
+        BuildADTRefinements QueryQSSpecs InsertQSSpecs EmptyQSSpecs
+        QueryStructure GeneralInsertRefinements
+        GeneralQueryRefinements ProcessScheduler.SetEq
+        ProcessScheduler.AdditionalLemmas
+        ListInsertRefinements ListQueryRefinements.
+
+Instance EnsembleListEquivalence_SiR {A}:
+  @UnConstrRelationSiRClass A (list A) :=
+  {| UnConstrRelationSiR := @EnsembleListEquivalence A |}.
+
+  Lemma EnsembleListEquivalence_Empty :
+    forall qsSchema Ridx,
+      EnsembleListEquivalence
+        (GetUnConstrRelation (DropQSConstraints (QSEmptySpec qsSchema))
+                             Ridx) [].
+  Proof.
+    intros; rewrite GetRelDropConstraints; simpl; split; simpl; intros;
+    unfold GetRelation, In in *;
+    rewrite Build_EmptyRelation_IsEmpty in *; simpl in *; auto.
+  Qed.
+
+Ltac implement_empty_list constrName RepSiR :=
+  hone constructor constrName;
+  [ unfold RepSiR, DropQSConstraints_SiR;
+    repeat setoid_rewrite refineEquiv_pick_ex_computes_to_and;
+    repeat setoid_rewrite refineEquiv_pick_eq';
+    simplify with monad laws;
+    repeat rewrite refineEquiv_pick_pair;
+    repeat (rewrite refine_pick_val;
+            [simplify with monad laws
+            | apply EnsembleListEquivalence_Empty]);
+        subst_body; higher_order_1_reflexivity
+  | ].
+
+Tactic Notation "implement" "using" "lists" "under" constr(Rep_SiR) :=
+    let SiR_Hyp := fresh in
+    pose Rep_SiR as SiR_Hyp;
+      unfold Rep_SiR in SiR_Hyp;
+      hone representation using SiR_Hyp;
+      repeat match goal with
+                 |- context[
+                        (const ?R ( _ : _ ) : rep :=
+                           { _ | exists _, _ })%consDef] =>
+                 implement_empty_list R SiR_Hyp
+             end;
+      repeat
+        match goal with
+            |- context [ (meth ?R ( _ : rep , _ : _ ) : _ :=
+                            {nr' | forall or , _ } )%methDef] =>
+            first [ implement insert in R with lists under SiR_Hyp
+                  | implement query in R with lists under SiR_Hyp ]
+        end.
