ADTExamples/QueryStructure/QueryStructureNotations.v
@@ -1,0 +1,16 @@
+Require Import String Omega List FunctionalExtensionality Ensembles
+        Computation ADT ADTRefinement ADTNotation QueryStructureSchema
+        BuildADTRefinements QueryQSSpecs InsertQSSpecs EmptyQSSpecs
+        QueryStructure GeneralInsertRefinements ListInsertRefinements
+        GeneralQueryRefinements ListQueryRefinements
+        ProcessScheduler.AdditionalLemmas.
+
+Open Scope QSSchema.
+Open Scope ADTSig.
+Open Scope QueryImpl.
+Open Scope QueryStructure.
+Open Scope Schema.
+Open Scope QuerySpec.
+Open Scope string.
+Open Scope Tuple.
+Open Scope comp_scope.
